More work on dafny4 tests

Test/dafny0/NewtypesResolution.dfy
@@ -398,28 +398,28 @@ module FunctionByMethod {
   // --- constraints
 
   newtype NT0 = x: int | P0(x)  // error: recursive dependency
-  ghost predicate P0(x: int) {
+  predicate P0(x: int) {
     x as NT0 == 3
   } by method {
     return x == 3;
   }
 
   newtype NT1 = x: int | P1(x)
-  ghost predicate P1(x: int) {
+  predicate P1(x: int) {
     x == 3
   } by method {
     return x as NT1 == 3;
   }
 
   type ST0 = x: int | Q0(x)  // error: recursive dependency
-  ghost predicate Q0(x: int) {
+  predicate Q0(x: int) {
     x as ST0 == 3
   } by method {
     return x == 3;
   }
 
   type ST1 = x: int | Q1(x)
-  ghost predicate Q1(x: int) {
+  predicate Q1(x: int) {
     x == 3
   } by method {
     return x as ST1 == 3;
@@ -428,56 +428,56 @@ module FunctionByMethod {
   // witnesses
 
   newtype NW0 = x: int | true ghost witness NWitness0()  // error: recursive dependency
-  ghost function NWitness0(): int {
+  function NWitness0(): int {
     150 + (0 as NW0 as int)
   } by method {
     return 150;
   }
 
   newtype NW1 = x: int | true ghost witness NWitness1()
-  ghost function NWitness1(): int {
+  function NWitness1(): int {
     150
   } by method {
     return 150 + (0 as NW1 as int);
   }
 
   newtype NW2 = x: int | true witness NWitness2()  // error: recursive dependency
-  ghost function NWitness2(): int {
+  function NWitness2(): int {
     150 + (0 as NW2 as int)
   } by method {
     return 150;
   }
 
   newtype NW3 = x: int | true witness NWitness3()  // error: recursive dependency
-  ghost function NWitness3(): int {
+  function NWitness3(): int {
     150
   } by method {
     return 150 + (0 as NW3 as int);
   }
 
   type SW0 = x: int | true ghost witness SWitness0()  // error: recursive dependency
-  ghost function SWitness0(): int {
+  function SWitness0(): int {
     150 + (0 as SW0 as int)
   } by method {
     return 150;
   }
 
   type SW1 = x: int | true ghost witness SWitness1()
-  ghost function SWitness1(): int {
+  function SWitness1(): int {
     150
   } by method {
     return 150 + (0 as SW1 as int);
   }
 
   type SW2 = x: int | true witness SWitness2()  // error: recursive dependency
-  ghost function SWitness2(): int {
+  function SWitness2(): int {
     150 + (0 as SW2 as int)
   } by method {
     return 150;
   }
 
   type SW3 = x: int | true witness SWitness3()  // error: recursive dependency
-  ghost function SWitness3(): int {
+  function SWitness3(): int {
     150
   } by method {
     return 150 + (0 as SW3 as int);
@@ -486,21 +486,21 @@ module FunctionByMethod {
   // constants
 
   ghost const c0 := R0()  // error: recursive dependency
-  ghost function R0(): int {
+  function R0(): int {
     2 + c0
   } by method {
     return 2;
   }
 
   const c1 := R1()  // error: recursive dependency
-  ghost function R1(): int {
+  function R1(): int {
     2 + c1
   } by method {
     return 2;
   }
 
   const c2 := R2()  // error: recursive dependency
-  ghost function R2(): int {
+  function R2(): int {
     2
   } by method {
     return 2 + c2;
