Test/git-issues/git-issue-1564-3to4.dfy
@@ -4,22 +4,22 @@
 // RUN: %diff "%s.expect" "%t"
 
 ghost function F0(): int
-function F1(): int
+function method F1(): int
 
 twostate function G0(): int
 
-ghost function H0(): int {
+function H0(): int {
   2
 } by method {
   return 2;
 }
 
 ghost predicate P0()
-predicate P1()
+predicate method P1()
 
 twostate predicate Q0()
 
-ghost predicate R0() {
+predicate R0() {
   true
 } by method {
   return true;
