Test/git-issues/git-issue-3410/git-issue-3410dd.dfy
@@ -1,0 +1,7 @@
+// RUN: %testDafnyForEachCompiler -- /compile:4 /noVerify "%s" > "%t"
+
+method Main() {
+  var i: int := 42;
+  assert {:expect} i == 41;
+  print "Done\n";
+}
