Test/git-issues/git-issue-3460/git-issue-3460a.dfy
@@ -1,0 +1,6 @@
+// RUN: %baredafny run --quiet:1 "%s" > "%t"
+// RUN: %diff "%s.expect" "%t"
+
+method Main() {
+  print "Done\n";
+}
